EffectSSA/ProofSketch/EqnInv.lean
@@ -1,5 +1,6 @@
 module
 
+public import EffectSSA.ProofSketch.Assumptions
 public import EffectSSA.ProofSketch.ProofSketch
 
 namespace EffectSSA.ProofSketch
@@ -18,9 +19,27 @@ section Axioms
 The semantics of an instruction may depend only on those variable declared
 as arguments.
 -/
-axiom denote_eq_of_args : ∀ i : Inst ι, ∀ ρ η : SEnv ι,
-  ρ.state = η.state → (∀ x ∈ i.args, ρ.locals x = η.locals x)
-  → ⟦i⟧ ρ = ⟦i⟧ η
+theorem denote_eq_of_args : ∀ i : Inst ι, ∀ ρ η : SEnv ι,
+    ρ.state = η.state → ρ.error = η.error →
+    (∀ x ∈ i.args, ρ.locals x = η.locals x)
+    → let ρ' := ⟦i⟧ ρ
+      let η' := ⟦i⟧ η
+      ρ'.state = η'.state
+      ∧ ∀ x ∈ i.results, ρ'.locals x = η'.locals x := by
+  rintro i ⟨ℓ₁, s₁, e₁⟩ ⟨ℓ₂, s₂, e₂⟩ rfl rfl hx
+  simp only at hx
+  have : List.mapM ℓ₂ i.args = List.mapM ℓ₁ i.args := by
+    revert hx; induction i.args <;> grind
+  simp only [denote_eq, Option.bind_eq_bind, this]
+  cases List.mapM ℓ₁ i.args
+  · simp
+  · rename_i args_vals
+    simp only [Option.bind_some]
+    obtain ⟨state', rs⟩ := ⟦i.opCode⟧ s₁ args_vals
+    simp only [LocalEnv.with?, bne_iff_ne, ne_eq, ite_not, Option.pure_def]
+    split
+    · simp; grind
+    · grind
 
 end Axioms
 
@@ -67,7 +86,7 @@ theorem purelyDet_imp (i : Inst ι) :
   intro pu ρ η hy x hx
   let η' : SEnv ι := { ρ with locals := η.locals }
   calc (⟦i⟧ ρ).locals x
-    _ = (⟦i⟧ η').locals x := by grind [denote_eq_of_args]
+    _ = (⟦i⟧ η').locals x := by have := denote_eq_of_args i ρ η'; grind only
     _ = (⟦i⟧ η).locals x := by grind [PurelyDet]
 
 /--
